CleanQ/CleanQ_SetListRefinement.thy
@@ -19,47 +19,48 @@ theory CleanQ_SetListRefinement imports
 begin
 
 
-definition sr_set_list :: "'a CleanQ_List_State \<Rightarrow> 'a CleanQ_Set_State"
-  where "sr_set_list st_c = \<lparr>SX = lSX st_c, SY = lSY st_c, 
-                             TXY = set (lTXY st_c), TYX = set (lTYX st_c)\<rparr>"
-
-definition fr_id :: "'a CleanQ_List_State \<Rightarrow> 'a CleanQ_Set_State"
-  where "fr_id = sr_set_list"
 
 lemma
   CleanQ_setListRefinement_enq_x: "((\<Gamma>a, CleanQ_Set_enq_x_pre K buf, Language.Basic (CleanQ_Set_enq_x buf)), 
                                (\<Gamma>c, CleanQ_List_enq_x_pre K buf, Language.Basic (CleanQ_List_enq_x buf)))
-                               \<in> refinement_s (separable_lift sr_set_list fr_id)"
+                               \<in> refinement_s (separable_lift CleanQ_List2Set CleanQ_List2Set)"
 apply(rule refinement_s_BasicI) (* Problem applying this after unfolding*)
-  unfolding separable_lift_def sr_set_list_def CleanQ_Set_enq_x_def CleanQ_Set_enq_x_pre_def CleanQ_List_enq_x_def
+  unfolding separable_lift_def CleanQ_List2Set_def CleanQ_Set_enq_x_def CleanQ_Set_enq_x_pre_def CleanQ_List_enq_x_def
   CleanQ_List_enq_x_pre_def
   by(auto)
 
 lemma
   CleanQ_setListRefinement_enq_y: "((\<Gamma>a, CleanQ_Set_enq_y_pre K buf, Language.Basic (CleanQ_Set_enq_y buf)), 
                                (\<Gamma>c, CleanQ_List_enq_y_pre K buf, Language.Basic (CleanQ_List_enq_y buf)))
-                               \<in> refinement_s (separable_lift sr_set_list fr_id)"
-apply(rule refinement_s_BasicI) (* Problem applying this after unfolding*)
-  unfolding separable_lift_def sr_set_list_def  CleanQ_Set_enq_y_def CleanQ_Set_enq_y_pre_def CleanQ_List_enq_y_def
+                               \<in> refinement_s (separable_lift CleanQ_List2Set CleanQ_List2Set)"
+  apply(rule refinement_s_BasicI) (* Problem applying this after unfolding*)
+   unfolding separable_lift_def CleanQ_List2Set_def  CleanQ_Set_enq_y_def CleanQ_Set_enq_y_pre_def CleanQ_List_enq_y_def
   CleanQ_List_enq_y_pre_def
   by(auto)
 
 lemma
   CleanQ_setListRefinement_deq_x: "((\<Gamma>a, CleanQ_Set_deq_x_pre K buf, Language.Basic (CleanQ_Set_deq_x buf)), 
-                               (\<Gamma>c, CleanQ_List_deq_x_pre K buf, Language.Basic (CleanQ_List_deq_x buf)))
-                               \<in> refinement_s (separable_lift sr_set_list fr_id)"
-apply(rule refinement_s_BasicI) (* Problem applying this after unfolding*)
-  unfolding separable_lift_def sr_set_list_def CleanQ_Set_deq_x_def CleanQ_Set_deq_x_pre_def CleanQ_List_deq_x_def
-  CleanQ_List_deq_x_pre_def
+                               (\<Gamma>c, CleanQ_List_deq_x_pre K buf, Language.Basic (CleanQ_List_deq_x)))
+                               \<in> refinement_s (separable_lift CleanQ_List2Set CleanQ_List2Set)"
+  apply(rule refinement_s_BasicI) (* Problem applying this after unfolding*)
+    unfolding separable_lift_def  CleanQ_Set_deq_x_def CleanQ_Set_deq_x_pre_def CleanQ_List_deq_x_def
+   CleanQ_List_deq_x_pre_def
+   apply(auto)
+ unfolding CleanQ_List2Set_def  
+   apply(simp add:list_set_hd_tl_subtract)
   by(auto)
+  
 
 lemma
   CleanQ_setListRefinement_deq_y: "((\<Gamma>a, CleanQ_Set_deq_y_pre K buf, Language.Basic (CleanQ_Set_deq_y buf)), 
-                               (\<Gamma>c, CleanQ_List_deq_y_pre K buf, Language.Basic (CleanQ_List_deq_y buf)))
-                               \<in> refinement_s (separable_lift sr_set_list fr_id)"
+                               (\<Gamma>c, CleanQ_List_deq_y_pre K buf, Language.Basic (CleanQ_List_deq_y)))
+                               \<in> refinement_s (separable_lift CleanQ_List2Set CleanQ_List2Set)"
 apply(rule refinement_s_BasicI) (* Problem applying this after unfolding*)
-  unfolding separable_lift_def sr_set_list_def CleanQ_Set_deq_y_def CleanQ_Set_deq_y_pre_def CleanQ_List_deq_y_def
+  unfolding separable_lift_def  CleanQ_Set_deq_y_def CleanQ_Set_deq_y_pre_def CleanQ_List_deq_y_def
   CleanQ_List_deq_y_pre_def
+   apply(auto)
+  unfolding CleanQ_List2Set_def
+   apply(simp add:list_set_hd_tl_subtract)
   by(auto)
-
+  
 end
